Issue 228: Fixed a bug in which the Cam was not exporting its register dependencies.

Cam/Ifc.v
@@ -22,6 +22,7 @@ Section cam.
   
     Class Cam
       := {
+           regs: list RegInitT;
            read: forall ty, keyK @# ty -> readCtxtK @# ty -> ActionT ty (Maybe dataK);
            write: forall ty, keyK @# ty -> dataK @# ty -> ActionT ty Void;
            flush: forall ty, ActionT ty Void;
